compiler/wasm/add_carryScript.sml
@@ -1,5 +1,5 @@
 Theory add_carry
-Ancestors words arithmetic integer_word
+Ancestors words arithmetic integer_word word_lemmas
 Libs wordsLib
 
 Definition add_carry_def:
@@ -68,28 +68,6 @@ Proof
   >-(dxrule_then assume_tac add_carry_aux'>>gvs[word_add_def])
 QED
 
-Theorem word_bits_1bit:
-  (i--i)a = if word_bit i a then 1w else 0w
-Proof
-  Cases_on `dimindex(:'a)<=i`
-  >-simp[WORD_BIT_BITS,WORD_BITS_ZERO3]
-  >>`∃n. a = n2w n` by metis_tac[n2w_w2n]
-  >>gvs[]
-  >>simp[word_bit_n2w,bitTheory.BIT_def,word_bits_n2w,MIN_DEF]
-  >>`(if i < dimindex (:α) − 1 then i else (dimindex (:α) − 1)) = i` by (IF_CASES_TAC>>gvs[])
-  >>pop_assum(fn eq=>simp[eq])
-  >>`BITS i i n = if BITS i i n = 1 then 1 else 0` suffices_by metis_tac[n2w_11]
-  >>metis_tac[bitTheory.BIT_def,bitTheory.NOT_BIT]
-QED
-
-Theorem lsr_msb:
-  a:'a word >>> (dimindex(:'a)-1) = if word_msb a then 1w else 0w
-Proof
-  simp[word_lsr_n2w,word_msb_def,word_bits_1bit]
-  >>`dimindex(:'a)-1<dimindex(:'a)` by simp[DIMINDEX_GT_0]
-  >>metis_tac[word_bit]
-QED
-
 Definition add_overflow_def:
   add_overflow (a:'a word) (b:'a word) =
   let sum = a+b in
@@ -101,14 +79,6 @@ Definition sub_overflow_def:
   let diff = a-b in
   (diff, ((a⊕b) && ~(b⊕diff)) >>> (dimindex(:'a)-1))
 End
-
-Theorem word_msb_xor:
-  word_msb(a⊕b) = ¬(word_msb a ⇔ word_msb b)
-Proof
-  simp[word_msb_def,word_bit]
-  >>`∃na nb. a = n2w na ∧ b = n2w nb` by metis_tac[n2w_w2n]
-  >>gvs[word_xor_n2w,word_bit_n2w,bitTheory.BITWISE_THM]
-QED
 
 Theorem add_overflow_thm:
   add_overflow a b = (sum, ovf) ⇒
