compiler/wasm/word_lemmasScript.sml
@@ -2,13 +2,37 @@ Theory word_lemmas
 Ancestors words arithmetic integer_word
 Libs wordsLib
 
-Theorem a:
-  a && m = a ==> a <=+ m
+Theorem word_bits_1bit:
+  (i--i)a = if word_bit i a then 1w else 0w
 Proof
-cheat
+  Cases_on `dimindex(:'a)<=i`
+  >-simp[WORD_BIT_BITS,WORD_BITS_ZERO3]
+  >>`∃n. a = n2w n` by metis_tac[n2w_w2n]
+  >>gvs[]
+  >>simp[word_bit_n2w,bitTheory.BIT_def,word_bits_n2w,MIN_DEF]
+  >>`(if i < dimindex (:α) − 1 then i else (dimindex (:α) − 1)) = i` by (IF_CASES_TAC>>gvs[])
+  >>pop_assum(fn eq=>simp[eq])
+  >>`BITS i i n = if BITS i i n = 1 then 1 else 0` suffices_by metis_tac[n2w_11]
+  >>metis_tac[bitTheory.BIT_def,bitTheory.NOT_BIT]
 QED
 
-Theorem c:
+Theorem lsr_msb:
+  a:'a word >>> (dimindex(:'a)-1) = if word_msb a then 1w else 0w
+Proof
+  simp[word_lsr_n2w,word_msb_def,word_bits_1bit]
+  >>`dimindex(:'a)-1<dimindex(:'a)` by simp[DIMINDEX_GT_0]
+  >>metis_tac[word_bit]
+QED
+
+Theorem word_msb_xor:
+  word_msb(a⊕b) = ¬(word_msb a ⇔ word_msb b)
+Proof
+  simp[word_msb_def,word_bit]
+  >>`∃na nb. a = n2w na ∧ b = n2w nb` by metis_tac[n2w_w2n]
+  >>gvs[word_xor_n2w,word_bit_n2w,bitTheory.BITWISE_THM]
+QED
+
+Theorem word_and_pow2m1_aux:
   n < dimindex(:'a) /\ 0<n ==>
   a:'a word && n2w(2**n-1) = (n-1><0) a
 Proof
@@ -16,14 +40,14 @@ Proof
 >>simp[word_extract_mask, n2w_sub, GSYM word_1_lsl]
 QED
 
-Theorem b:
+Theorem word_and_pow2m1:
   n < dimindex(:'a) /\
   a:'a word <+ n2w(2**n) ==>
   a && n2w(2**n-1) = a
 Proof
-`?na. a = n2w na /\ na < dimword(:'a)` by cheat(*metis_tac[n2w_w2n]*)
+`∃na. a = n2w na /\ na < dimword(:'a)` by metis_tac[n2w_w2n,w2n_lt]
 >>Cases_on‘n’>-simp[word_lo_n2w]
->>rw[c,word_extract_n2w,MIN_DEF,bitTheory.BITS_ZERO3,word_lo_n2w,dimword_def]
+>>rw[word_and_pow2m1_aux,word_extract_n2w,MIN_DEF,bitTheory.BITS_ZERO3,word_lo_n2w,dimword_def]
 >>gvs[]
->>metis_tac[EXP_BASE_LT_MONO,LESS_TRANS,prove(``1n<2``,simp[])]
+>>metis_tac[EXP_BASE_LT_MONO,LESS_TRANS,prove(“1n<2”,simp[])]
 QED
